Use Block instead of BlockHeader in state_transition.

src/dafny/beacon/StateTransition.dfy
@@ -140,6 +140,26 @@ module StateTransition {
             )
     }
 
+    predicate isValid2(s : BeaconState, b : BeaconBlock) 
+    {
+        //  block slot should be in the future.
+        s.slot < b.slot 
+        //  Fast forward s to b.slot and check `b` can be attached to the
+        //  resulting state's latest_block_header.
+        && b.parent_root == 
+            hash_tree_root(
+                forwardStateToSlot(resolveStateRoot(s), 
+                b.slot
+            ).latest_block_header) 
+        //  Check that the block provides the correct hash for the state.
+        &&  b.state_root == hash_tree_root(
+                addBlockToState2(
+                    forwardStateToSlot(resolveStateRoot(s), b.slot), 
+                    b
+                )
+            )
+    }
+
     /**
      *  Compute the state obtained after adding a block.
      *  
@@ -178,6 +198,36 @@ module StateTransition {
         assert (b.state_root == hash_tree_root(s'));
     }  
 
+     method stateTransition2(s: BeaconState, b: BeaconBlock) returns (s' : BeaconState)
+        //  make sure the last state was one right after addition of new block
+        requires isValid2(s, b)
+
+        /** The next state latest_block_header is same as b except for state_root that is 0. */
+        ensures s'.latest_block_header == BeaconBlockHeader(b.slot, b.parent_root, EMPTY_BYTES32)
+        /** s' slot is now adjusted to the slot of b. */
+        ensures s'.slot == b.slot
+        /** s' parent_root is the hash of the state obtained by resolving/forwarding s to
+            the slot of b.  */
+        ensures s'.latest_block_header.parent_root  == 
+            hash_tree_root(
+                forwardStateToSlot(resolveStateRoot(s), b.slot)
+                .latest_block_header
+            )
+    {
+        //  finalise slots before b.slot.
+        var s1 := processSlots(s, b.slot);
+
+        //  Process block and compute the new state.
+        s' := processBlock2(s1, b);  
+
+        // Verify state root (from eth2.0 specs)
+        // A proof that this function is correct establishes that this assert statement 
+        // is never violated (i.e. when isValid() is true.)
+        // In the Eth2.0 specs this check is conditional and enabled by default.
+        //  if validate_result:
+        assert (b.state_root == hash_tree_root(s'));
+    }  
+
     /**
      *  Advance current state to a given slot.
      *
@@ -196,14 +246,11 @@ module StateTransition {
      *                  proposed block.
      *  @returns        The state obtained after advancing the histories to slot.
      *      
-     *  @note          The specs have the the first processSlot integrated
-     *                  in the while loop. However, because s.slot < slot,
-     *                  the while bdoy must be executed at least one time.
-     *                  To simplify the proof, we have taken this first iteration
-     *                  outside of the loop. It does not change the semantics
-     *                  but enables us to use the state obtained after the first
-     *                  iteration the loop and prove it is the same as 
-     *                  resolveStateRoot(s); 
+     *  @note           The specs have the the first processSlot integrated in the while loop. However, 
+     *                  because s.slot < slot, the while bdoy must be executed at least one time.
+     *                  To simplify the proof, we have taken this first iteration outside of the loop. It does 
+     *                  not change the semantics but enables us to use the state obtained after the first
+     *                  iteration the loop and prove it is the same as resolveStateRoot(s).
      *
      */
     method processSlots(s: BeaconState, slot: Slot) returns (s' : BeaconState)
@@ -312,6 +359,20 @@ module StateTransition {
         //  process_operations(s, b.body)
     }
 
+     method processBlock2(s: BeaconState, b: BeaconBlock) returns (s' : BeaconState) 
+        requires b.slot == s.slot
+        requires b.parent_root == hash_tree_root(s.latest_block_header)
+
+        ensures s' == addBlockToState2(s, b)
+    {
+        //  Start by creating a block header from the ther actual block.
+        s' := processBlockHeader2(s, b); 
+        
+        //  process_randao(s, b.body)
+        //  process_eth1_data(s, b.body)
+        //  process_operations(s, b.body)
+    }
+
     /**
      *  Check whether a block is valid and prepare and initialise new state
      *  with a corresponding block header. 
@@ -329,6 +390,23 @@ module StateTransition {
         requires b.parent_root == hash_tree_root(s.latest_block_header) 
 
         ensures s' == addBlockToState(s, b)
+    {
+        s':= s.(
+            latest_block_header := BeaconBlockHeader(
+                b.slot,
+                b.parent_root,
+                EMPTY_BYTES32
+            )
+        );
+    }
+
+    method processBlockHeader2(s: BeaconState, b: BeaconBlock) returns (s' : BeaconState) 
+        //  Verify that the slots match
+        requires b.slot == s.slot  
+        // Verify that the parent matches
+        requires b.parent_root == hash_tree_root(s.latest_block_header) 
+
+        ensures s' == addBlockToState2(s, b)
     {
         s':= s.(
             latest_block_header := BeaconBlockHeader(
@@ -363,6 +441,21 @@ module StateTransition {
      *  @returns    The state `s` updated to point to `b` with state_root set to 0.
      */
     function addBlockToState(s: BeaconState, b: BeaconBlockHeader) :  BeaconState 
+        //  Verify that the slots match
+        requires b.slot == s.slot  
+        // Verify that the parent matches
+        requires b.parent_root == hash_tree_root(s.latest_block_header) 
+    {
+        s.(
+            latest_block_header := BeaconBlockHeader(
+                b.slot,
+                b.parent_root,
+                EMPTY_BYTES32
+            )
+        )
+    }
+
+    function addBlockToState2(s: BeaconState, b: BeaconBlock) :  BeaconState 
         //  Verify that the slots match
         requires b.slot == s.slot  
         // Verify that the parent matches
